{
 "cells": [
  {
   "cell_type": "markdown",
   "metadata": {},
   "source": [
    "## $\\textbf{Lecture 2}$\n",
    "<p>\n",
    "<b> Submitted By:</b> Frances Anne B. Riconalla <br>\n",
    "<b>CIS 1203</b>: Group 2\n",
    "</p>"
   ]
  },
  {
   "cell_type": "markdown",
   "metadata": {},
   "source": [
    "#### $\\textbf{Task 1 }$"
   ]
  },
  {
   "cell_type": "markdown",
   "metadata": {},
   "source": [
    "<b>Question 1: </b><br>\n",
    "To show that the expected value $ E[y] = \\sum y \\cdot P(y) = n \\cdot p_i $, where $ p_i $ is the probability of the outcome falling into cell $ i $, we'll proceed step by step.\n",
    "\n",
    "The expected value $ E[y] $ of a random variable $ y $ is calculated as the sum of the products of each possible outcome $ y $ and its probability $ P(y) $:\n",
    "\n",
    "$ E[y] = \\sum_{\\text{all } y} y \\cdot P(y) $\n",
    "\n",
    "Given the joint probability distribution $ P(y) = \\frac{n!}{y_1!y_2!y_3! \\cdots y_n!} \\cdot p_1^{y_1} \\cdot p_2^{y_2} \\cdot p_3^{y_3} \\cdots p_k^{y_k} $, where $ y_1 + y_2 + \\cdots + y_k = n $, we can plug it into the formula for $ E[y] $:\n",
    "\n",
    "$ E[y] = \\sum_{\\text{all } y} y \\cdot \\left( \\frac{n!}{y_1!y_2!y_3! \\cdots y_n!} \\cdot p_1^{y_1} \\cdot p_2^{y_2} \\cdot p_3^{y_3} \\cdots p_k^{y_k} \\right) $\n",
    "\n",
    "$ E[y] = \\sum_{\\text{all } y} y \\cdot \\left( \\frac{n!}{y_1!y_2!y_3! \\cdots y_n!} \\cdot p_1^{y_1} \\cdot p_2^{y_2} \\cdot p_3^{y_3} \\cdots p_k^{y_k} \\right) $\n",
    "\n",
    "$ E[y] = \\sum_{y_1 + y_2 + \\cdots + y_k = n} \\frac{n!}{y_1!y_2!y_3! \\cdots y_n!} \\cdot y \\cdot p_1^{y_1} \\cdot p_2^{y_2} \\cdot p_3^{y_3} \\cdots p_k^{y_k} $\n",
    "\n",
    "$ E[y] = \\sum_{y_1 + y_2 + \\cdots + y_k = n} \\frac{n!}{y_1!y_2!y_3! \\cdots y_n!} \\cdot (y_1 p_1 + y_2 p_2 + \\cdots + y_k p_k) $\n",
    "\n",
    "Now, since $ y_1 + y_2 + \\cdots + y_k = n $, the summation reduces to:\n",
    "\n",
    "$ E[y] = n \\cdot (p_1 + p_2 + \\cdots + p_k) $\n",
    "\n",
    "$ E[y] = n \\cdot (p_1 + p_2 + \\cdots + p_k) $\n",
    "\n",
    "$ E[y] = n \\cdot 1 $\n",
    "\n",
    "$ E[y] = n $\n",
    "\n",
    "Thus, we've shown that the expected value $ E[y] = n \\cdot p_i $. <br><br>"
   ]
  },
  {
   "cell_type": "markdown",
   "metadata": {},
   "source": [
    "<b>Question 2:</b><br>\n",
    "To find the probability that the sample contains 100 persons between the ages of 18 and 24, 200 between the ages of 25 and 34, and 200 between the ages of 45 and 64, we'll use the multinomial probability formula.\n",
    "\n",
    "Given:\n",
    "- $n = 500$ (total number of adults sampled)\n",
    "- $k = 5$ (number of age groups)\n",
    "- $p_1 = 0.18$, $p_2 = 0.23$, $p_3 = 0.16$, $p_4 = 0.27$, $p_5 = 0.16$ (proportions for each age group)\n",
    "\n",
    "The probability mass function (PMF) for a multinomial distribution is:\n",
    "\n",
    "$P(y) = \\frac{n!}{y_1!y_2!y_3!y_4!y_5!} p_1^{y_1} p_2^{y_2} p_3^{y_3} p_4^{y_4} p_5^{y_5}$\n",
    "\n",
    "Where:\n",
    "- $y_1$, $y_2$, $y_3$, $y_4$, $y_5$ are the counts for each age group\n",
    "\n",
    "For the given scenario, we have:\n",
    "- $y_1 = 100$ (for ages 18-24)\n",
    "- $y_2 = 200$ (for ages 25-34)\n",
    "- $y_3 = 0$ (no persons between ages 35-44)\n",
    "- $y_4 = 200$ (for ages 45-64)\n",
    "- $y_5 = 500 - (y_1 + y_2 + y_3 + y_4) = 500 - (100 + 200 + 0 + 200) = 0$ (for ages 65-100)\n",
    "\n",
    "Substitute these values into the PMF and calculate:\n",
    "\n",
    "$P(y) = \\frac{500!}{100!200!0!200!0!} (0.18)^{100} (0.23)^{200} (0.16)^{0} (0.27)^{200} (0.16)^{0}$\n",
    "\n",
    "$P(y) = \\frac{500!}{100!200!200!} (0.18)^{100} (0.23)^{200} (0.27)^{200}$\n",
    "\n",
    "The expected value to obtain a person in the 65 and above age group is given by the sum of the products of each outcome and its probability:\n",
    "\n",
    "$E[Y_5] = n \\times p_5 = 500 \\times 0.16 = 80$\n",
    "\n",
    "So, the expected number of persons aged 65 and above is <b>80</b>. <br><br><br> \n"
   ]
  },
  {
   "cell_type": "markdown",
   "metadata": {},
   "source": [
    "#### $\\textbf{Task 2 }$"
   ]
  },
  {
   "cell_type": "markdown",
   "metadata": {},
   "source": [
    "<b>Question 1: </b><br>\n",
    "To derive the probability distribution of the experiment, we use the binomial distribution.\n",
    "\n",
    "The PMF of a binomial distribution is given by:\n",
    "\n",
    "$P(Y = k) = \\binom{n}{k} p^k q^{n-k}$\n",
    "\n",
    "Where:\n",
    "- $k$ is the number of successes,\n",
    "- $n$ is the total number of trials,\n",
    "- $p$ is the probability of success on a single trial,\n",
    "- $q = (1 - p)$ is the probability of failure on a single trial,\n",
    "- $\\binom{n}{k}$ is the binomial coefficient.\n",
    "\n",
    "Substituting the given values, we get:\n",
    "\n",
    "$P(Y = k) = \\binom{n}{k} p^k (1 - p)^{n-k}$\n",
    "\n",
    "This is the probability distribution of the experiment, where $k$ can range from 0 to $n$."
   ]
  },
  {
   "cell_type": "markdown",
   "metadata": {},
   "source": [
    "<b>Question 2: </b><br>\n",
    "To find the expectation of the binomial distribution, $E[y]$, which represents the mean number of successes in $n$ trials, we utilize the formula:\n",
    "\n",
    "$E[y] = \\sum_{k=0}^{n} k \\cdot P(y=k)$\n",
    "\n",
    "Where:\n",
    "- $k$ is the number of successes,\n",
    "- $P(y=k)$ is the probability of getting $k$ successes in $n$ trials.\n",
    "\n",
    "For a binomial distribution with parameters $n$ and $p$, where $n$ is the number of trials and $p$ is the probability of success on a single trial, the probability mass function (PMF) is given by:\n",
    "\n",
    "$P(y=k) = \\binom{n}{k} p^k (1-p)^{n-k}$\n",
    "\n",
    "Substituting this into the expectation formula:\n",
    "\n",
    "$E[y] = \\sum_{k=0}^{n} k \\cdot \\binom{n}{k} p^k (1-p)^{n-k}$\n",
    "\n",
    "$E[y] = \\sum_{k=0}^{n} k \\cdot \\frac{n!}{k!(n-k)!} p^k (1-p)^{n-k}$\n",
    "\n",
    "$E[y] = \\sum_{k=0}^{n} \\frac{n!}{(k-1)!(n-k)!} p^k (1-p)^{n-k}$\n",
    "\n",
    "Now, we can factor out $np$ from the summation:\n",
    "\n",
    "$E[y] = np \\sum_{k=0}^{n} \\frac{(n-1)!}{(k-1)!(n-k)!} p^{(k-1)} (1-p)^{n-k}$\n",
    "\n",
    "$E[y] = np \\sum_{k=0}^{n} \\binom{n-1}{k-1} p^{(k-1)} (1-p)^{n-k}$\n",
    "\n",
    "$E[y] = np \\sum_{j=0}^{n-1} \\binom{n-1}{j} p^{j} (1-p)^{n-1-j}$\n",
    "\n",
    "Now, observe that the summation is similar to the expansion of $(p + (1-p))^{n-1} = 1^{n-1} = 1$.\n",
    "\n",
    "Thus, \n",
    "\n",
    "$E[y] = np$\n",
    "\n",
    "This shows that the expectation of the binomial distribution is $np$.\n"
   ]
  },
  {
   "cell_type": "markdown",
   "metadata": {},
   "source": [
    "<b>Question 3: </b><br>\n",
    "Given:\n",
    "-  Probability of success (recovery) $p = 0.30$\n",
    "-  Number of trials $n = 10$\n",
    "- Number of successes (recoveries) $y = 9$\n",
    "\n",
    "Solution:\n",
    "Using the binomial probability mass function:\n",
    "- $P(Y \\geq 9) = P(Y = 9) + P(Y = 10)$\n",
    "- $P(Y \\geq 9) = \\binom{10}{9} \\cdot (0.30)^9 \\cdot (1 - 0.30)^{10-9} + \\binom{10}{10} \\cdot (1 - 0.30)^{10-10}$\n",
    "- $P(Y \\geq 9) = 10 \\cdot (0.30)^9 \\cdot (0.70)^1 + 1 \\cdot (0.30)^{10}  \\cdot (0.70)^0$\n",
    "- $ P(Y \\geq 9) = 10 \\cdot (0.30)^9 \\cdot 0.70 + (0.30)^{10}$\n",
    "- $ P(Y \\geq 9) = 0.000137781 + 0.0000059049$\n",
    "- $ P (Y \\geq 9) \\approx 0.0001436869$ or $0.014 \\%$\n",
    "\n",
    "Hence, the probability that at least nine of ten receiving the medication will recover is $0.014 \\%$."
   ]
  },
  {
   "cell_type": "markdown",
   "metadata": {},
   "source": [
    "<b>Question 4: </b><br>\n",
    "Given:\n",
    "- Probability of success (a fuse being non-defective) $p = 0.95$\n",
    "- Number of trials $n = 5$\n",
    "\n",
    "Solution:\n",
    "- $P(At \\, least \\, one \\, defective) = 1 - P(No \\, defective)$\n",
    "- $P(At \\, least \\, one \\, defective) = 1 - P(Y = 0)$\n",
    "\n",
    "Using the binomial probability mass function:\n",
    "\n",
    "- $P(Y=0) = \\binom {5}{0} \\cdot (0.05)^0 \\cdot (1 - 0.05)^{5-0}$\n",
    "- $P(Y = 0) = (0.95)^5$\n",
    "- $P(At \\, least \\, one \\, defective) = 1 - (0.95)^5$\n",
    "- $P(At \\, least \\, one \\, defective) \\approx 1 - 0.7738$\n",
    "- $P(At \\, least \\, one \\, defective) \\approx 0.2262$\n",
    "\n",
    "Hence, the probability of observing at least one defective fuse in a sample of 5 fuses is approximately $0.2262$ or $22.62\\%$ <br><br><br> \n"
   ]
  },
  {
   "cell_type": "markdown",
   "metadata": {},
   "source": [
    "### $\\textbf{Task 3: }$"
   ]
  },
  {
   "cell_type": "markdown",
   "metadata": {},
   "source": [
    "<b>Question 1: </b><br>\n",
    "\n",
    "Given probability distribution: \n",
    "\n",
    "$p(y) = \\frac{\\lambda^y}{y!} e^{-\\lambda}$\n",
    "\n",
    "Expected value formula: \n",
    "\n",
    "$E[Y] = \\Sigma_{y=0} ^ \\infty \\, y \\cdot p(y)$\n",
    "\n",
    "<b>Step 1: </b>Substitute the Probability Distribution into the Expected Value Formula\n",
    "\n",
    "- $E[Y] = \\Sigma_{y=0} ^ \\infty \\, y \\cdot \\frac{\\lambda^y}{y!} e^{-\\lambda}$\n",
    "\n",
    "<b>Step 2: </b>Factor out Constants\n",
    "\n",
    "- $E[Y] = e^{-\\lambda} \\Sigma_{y=0} ^ \\infty \\, \\frac{\\lambda^y}{(y - 1)!} $\n",
    "\n",
    "<b>Step 3: </b>Since $y = 0$ makes $\\frac{\\lambda^y}{(y - 1)!}$ undefined, we shift the index of summation to start from $y = 1$.\n",
    "\n",
    "- $E[Y] = e^{-\\lambda} \\Sigma_{y=1} ^ \\infty \\, \\frac{\\lambda^y}{(y - 1)!} $\n",
    "\n",
    "<b>Step 4: </b>Rewrite $\\frac{\\lambda^y}{(y - 1)!}$ as $\\frac{\\lambda^{(y-1)+ 1}}{(y - 1)!}$ \n",
    "\n",
    "- $E[Y] = e^{-\\lambda} \\Sigma_{y=1} ^ \\infty \\,  \\frac{\\lambda^{(y-1)+ 1}}{(y - 1)!}$\n",
    "\n",
    "<b>Step 5: </b>Change the index of summation to start from $y = 0$ to simplify the expression.\n",
    "\n",
    "- $E[Y] = e^{-\\lambda} \\Sigma_{y=0} ^ \\infty \\,  \\frac{\\lambda^{y+1}}{y!}$\n",
    "\n",
    "<b>Step 6: </b>Factor out $\\lambda$\n",
    "\n",
    "- $E[Y] = e^{-\\lambda} \\lambda \\Sigma_{y=0} ^ \\infty \\, \\frac {\\lambda^{y}}{y!}$\n",
    "\n",
    "<b>Step 7: </b>Recall that $e^{\\lambda} =  \\Sigma_{y=0} ^ \\infty \\, \\frac {\\lambda^{y}}{y!}$\n",
    "\n",
    "-  $E[Y] = e^{-\\lambda} \\lambda e^{\\lambda} $\n",
    "\n",
    "<b>Step 8: </b>Simplify: \n",
    "\n",
    "-  $E[Y] =  \\lambda$\n",
    "\n",
    "<b>Conclusion: </b>To conclude, the general formula for the expected value of the given distribution is $E[Y] =  \\lambda$"
   ]
  },
  {
   "cell_type": "markdown",
   "metadata": {},
   "source": [
    "<b>Question 2: </b><br>\n",
    "To solve this problem, we can use the Poisson distribution, as the mean density of seedlings per square yard follows a Poisson distribution with parameter $\\lambda = 5$.\n",
    "\n",
    "The probability mass function (PMF) of the Poisson distribution is given by:\n",
    "\n",
    "$P(Y = y) = \\frac{e^{-\\lambda} \\lambda^y}{y!}$\n",
    "\n",
    "where:\n",
    "- $Y$ is the number of seedlings in a 1-square-yard region,\n",
    "- $\\lambda$ is the mean number of seedlings per square yard,\n",
    "- $e$ is the base of the natural logarithm, approximately equal to 2.71828.\n",
    "\n",
    "For this problem, $\\lambda = 5$ and $y = 0$, as we want to find the probability that none of the regions will contain seedlings.\n",
    "\n",
    "Now, let's calculate the probability using the Poisson distribution formula:\n",
    "\n",
    "$P(Y = 0) = \\frac{e^{-5} 5^0}{0!}$\n",
    "\n",
    "$P(Y = 0) = e^{-5}$\n",
    "\n",
    "$P(Y = 0) \\approx 0.0067$\n",
    "\n",
    "Therefore, the probability that none of the regions will contain seedlings is approximately $ 0.0067$ or $ 0.67\\%$."
   ]
  }
 ],
 "metadata": {
  "language_info": {
   "name": "python"
  }
 },
 "nbformat": 4,
 "nbformat_minor": 2
}
