{
 "cells": [
  {
   "cell_type": "markdown",
   "metadata": {},
   "source": [
    "<h1 style=\"font-weight:Bold\">Discrete Structures 2 Programming Assignments</h1>\n"
   ]
  },
  {
   "cell_type": "markdown",
   "metadata": {},
   "source": [
    "Siobhan B. Leonor TTH 12:00 - 1:30PM"
   ]
  },
  {
   "cell_type": "markdown",
   "metadata": {},
   "source": [
    "**<h2>Lecture 1:</h2>**"
   ]
  },
  {
   "cell_type": "markdown",
   "metadata": {},
   "source": [
    "\n",
    "**1. To prove that $e$ is irrational**\n",
    "\n",
    "we'll start by assuming the opposite, that $e$ is rational, meaning it can be expressed as a ratio of two integers $\\frac{a}{b}$, where $a$ and $b$ are integers with no common factors other than 1.\n",
    "\n",
    "Now, let's recall the series expansion of $e$:\n",
    "\n",
    "$$ e = \\sum_{k=0}^{\\infty} \\frac{1}{k!} = 1 + \\frac{1}{1!} + \\frac{1}{2!} + \\frac{1}{3!} + \\cdots $$\n",
    "\n",
    "Each term in this sum is positive, so if $e = \\frac{a}{b}$, then $\\frac{a}{b} > 0$, which means $a > 0$ and $b > 0$.\n",
    "\n",
    "Consider the sum of the first $n$ terms of the series for some large integer $n$, denoted as $S_n$:\n",
    "\n",
    "$$ S_n = 1 + \\frac{1}{1!} + \\frac{1}{2!} + \\cdots + \\frac{1}{n!} $$\n",
    "\n",
    "Since each term in this sum is positive, $S_n$ is an increasing sequence. Also, $S_n$ is bounded above by $e$, because $e$ is the limit of this sequence as $n$ approaches infinity.\n",
    "\n",
    "Now, let's choose $n$ such that $b > (n+1)!$. Since $b$ is finite, such an $n$ exists.\n",
    "\n",
    "If we multiply both sides of $e = \\frac{a}{b}$ by $(n+1)!$, we get:\n",
    "\n",
    "$$ (n+1)! \\cdot e = (n+1)! \\cdot \\frac{a}{b} = a \\cdot \\frac{(n+1)!}{b} $$\n",
    "\n",
    "Since $b > (n+1)!$, $\\frac{(n+1)!}{b} < 1$, so $a \\cdot \\frac{(n+1)!}{b}$ is less than $a$.\n",
    "\n",
    "Now, let's consider $(n+1)! \\cdot S_n$:\n",
    "\n",
    "$$ (n+1)! \\cdot S_n = (n+1)! + (n+1)! \\cdot \\frac{1}{1!} + \\cdots + (n+1)! \\cdot \\frac{1}{n!} $$\n",
    "\n",
    "Each term of this sum is less than $a$, and there are $a$ terms in total, so $(n+1)! \\cdot S_n < a \\cdot a = a^2$.\n",
    "\n",
    "Similarly, $(n+1)! \\cdot S_{n+1} > a$.\n",
    "\n",
    "So, we have $a < (n+1)! \\cdot S_n < a^2 < (n+1)! \\cdot S_{n+1} < a$. This is a contradiction, because $a$ is an integer.\n",
    "\n",
    "Therefore, our initial assumption that $e$ is rational must be false, and thus $e$ is irrational.\n"
   ]
  },
  {
   "cell_type": "markdown",
   "metadata": {},
   "source": [
    "**2. To prove Minkowski's Inequality for sums**\n",
    "\n",
    "Start with the expression:\n",
    "\n",
    "\\begin{equation}\n",
    "\\left( \\sum_{k=1}^{n} (a_{k} + b_{k})^p \\right)^{\\frac{1}{p}} \\leq \\left( \\sum_{k=1}^{n} a_{k}^p \\right)^{\\frac{1}{p}} + \\left( \\sum_{k=1}^{n} b_{k}^p \\right)^{\\frac{1}{p}}\n",
    "\\end{equation}\n",
    "\n",
    "\n",
    "\\begin{align}\n",
    "\\sum_{k=1}^{n} (a_{k} + b_{k})^p &= \\sum_{k=1}^{n} a_{k}(a_{k} + b_{k})^{p-1} + \\sum_{k=1}^{n} b_{k}(a_{k} + b_{k})^{p-1} \\\\\n",
    "&\\leq \\left( \\sum_{k=1}^{n} a_{k}^p \\right)^{\\frac{1}{p}} \\left( \\sum_{k=1}^{n} (a_{k} + b_{k})^{p-1} \\right)^{\\frac{1}{q}} + \\left( \\sum_{k=1}^{n} b_{k}^p \\right)^{\\frac{1}{p}} \\left( \\sum_{k=1}^{n} (a_{k} + b_{k})^{p-1} \\right)^{\\frac{1}{q}}\n",
    "\\end{align}\n",
    "\n",
    "\\begin{align}\n",
    "&= \\left( \\sum_{k=1}^{n} a_{k}^p \\right)^{\\frac{1}{p}} \\left( \\sum_{k=1}^{n} (a_{k} + b_{k})^p \\right)^{\\frac{1}{q}} + \\left( \\sum_{k=1}^{n} b_{k}^p \\right)^{\\frac{1}{p}} \\left( \\sum_{k=1}^{n} (a_{k} + b_{k})^p \\right)^{\\frac{1}{q}} \\\\\n",
    "\n",
    "&\\text{Power of Power, and by hypothesis: } (p-1)q = p\n",
    "\\end{align}\n",
    "\n",
    "\n",
    "\\begin{equation}\n",
    "\\Rightarrow \\left( \\sum_{k=1}^{n} (a_{k} + b_{k})^p \\right)^{1-\\frac{1}{q}} \\leq \\left( \\sum_{k=1}^{n} a_{k}^p \\right)^{\\frac{1}{p}} + \\left( \\sum_{k=1}^{n} b_{k}^p \\right)^{\\frac{1}{p}}\n",
    "\\end{equation}\n",
    "\n",
    "\\begin{equation}\n",
    "\\Rightarrow \\left( \\sum_{k=1}^{n} (a_{k} + b_{k})^p \\right)^{\\frac{1}{p}} \\leq \\left( \\sum_{k=1}^{n} a_{k}^p \\right)^{\\frac{1}{p}} + \\left( \\sum_{k=1}^{n} b_{k}^p \\right)^{\\frac{1}{p}}\n",
    "\\end{equation}"
   ]
  },
  {
   "cell_type": "markdown",
   "metadata": {},
   "source": [
    "**3. To prove the triangle inequality:**\n",
    "\n",
    "\\begin{align*}\n",
    "\\lvert x + y \\rvert &\\leq \\lvert x \\rvert + \\lvert y \\rvert, \\quad \\forall (x,y) \\in \\mathbb{R} \\\\\n",
    "\\text{where } x &\\in \\mathbb{R}, \\text{ and} \\\\\n",
    "\\lvert x \\rvert &= \\max \\{ x, -x \\} = \\begin{cases} x & \\text{if } x \\geq 0 \\\\ -x & \\text{if } x \\leq 0 \\end{cases}\n",
    "\\end{align*}\n"
   ]
  },
  {
   "cell_type": "markdown",
   "metadata": {},
   "source": [
    "It follows that $x \\leq |x|$ and $-x \\leq |x|$.\n",
    "\n",
    "Now, let's fix $a, b \\in \\mathbb{R}$:\n",
    "\n",
    "$$\n",
    "\\begin{aligned}\n",
    "a + b &\\leq |a| + |b| \\\\\n",
    "- a -b &\\leq |a| + |b| \\\\\n",
    "- a - b &= -(a+b)\n",
    "\\end{aligned}\n",
    "$$\n",
    "\n",
    "So,\n",
    "\n",
    "$$\n",
    "\\begin{aligned}\n",
    "a+b &\\leq |a| + |b| \\\\\n",
    "-(a+b) &\\leq |a| + |b|\n",
    "\\end{aligned}\n",
    "$$\n",
    "\n",
    "$$\n",
    "\\max \\{ a + b, -(a+b) \\} = |a + b | \\leq |a| + |b|\n",
    "$$\n"
   ]
  },
  {
   "cell_type": "markdown",
   "metadata": {},
   "source": [
    "**4.**\n",
    "**Proof of Sedrakayan's Lemma:**\n",
    "\n",
    "We start by using the Cauchy-Schwarz Inequality.\n",
    "\n",
    "The Cauchy-Schwarz Inequality states that for any real numbers $a_1, a_2, ..., a_n$ and $b_1, b_2, ..., b_n$, the following inequality holds:\n",
    "\n",
    "$$\n",
    "\\left( \\sum_{i=1}^{n} a_i b_i \\right)^2 \\leq \\left( \\sum_{i=1}^{n} a_i^2 \\right) \\left( \\sum_{i=1}^{n} b_i^2 \\right)\n",
    "$$\n",
    "\n",
    "Let's use this inequality with $a_i = \\sqrt{v_i}$ and $b_i = \\frac{u_i}{\\sqrt{v_i}}$:\n",
    "\n",
    "$$\n",
    "\\left( \\sum_{i=1}^{n} \\sqrt{v_i} \\frac{u_i}{\\sqrt{v_i}} \\right)^2 \\leq \\left( \\sum_{i=1}^{n} (\\sqrt{v_i})^2 \\right) \\left( \\sum_{i=1}^{n} \\left( \\frac{u_i}{\\sqrt{v_i}} \\right)^2 \\right)\n",
    "$$\n",
    "\n",
    "This simplifies to:\n",
    "\n",
    "$$\n",
    "\\left( \\sum_{i=1}^{n} u_i \\right)^2 \\leq \\left( \\sum_{i=1}^{n} v_i \\right) \\left( \\sum_{i=1}^{n} \\frac{u_i^2}{v_i} \\right)\n",
    "$$\n",
    "\n",
    "Now, divide both sides by $\\sum_{i=1}^{n} v_i$:\n",
    "\n",
    "$$\n",
    "\\frac{\\left( \\sum_{i=1}^{n} u_i \\right)^2}{\\sum_{i=1}^{n} v_i} \\leq \\sum_{i=1}^{n} \\frac{u_i^2}{v_i}\n",
    "$$\n",
    "\n",
    "This proves Sedrakayan's Lemma.\n"
   ]
  },
  {
   "cell_type": "markdown",
   "metadata": {},
   "source": [
    "**1.**\n",
    "\n",
    " Consider the functions $ ( f(x) = 2x+1 ), ( g(x)=2y-1 ), ( j(x) = |f(x)+g(x)| ), and ( h(x) = j(x)^2 ). $ Show that:\n",
    "\n",
    "$$\n",
    "\\sqrt{|f(x)|^2} \\geq \\sqrt{h(x)} - \\sqrt{|g(x)|^2}, \\quad \\forall (x,y) \\in \\mathbb{Z}^+\n",
    "$$\n",
    "\n",
    "Find the expressions for $( |f(x)|^2 ) and ( |g(x)|^2 ):$\n",
    "\n",
    "\n",
    "\n",
    "$$\n",
    "|f(x)|^2 = |2x+1|^2 = (2x+1)^2\n",
    "$$\n",
    "\n",
    "$$\n",
    "|g(x)|^2 = |2y-1|^2 = (2y-1)^2\n",
    "$$\n",
    "\n",
    "Find the expression for \\( h(x) \\):\n",
    "\n",
    "$$\n",
    "j(x) = |f(x)+g(x)| = |(2x+1) + (2y-1)| = |2x + 2y| = 2|x + y|\n",
    "$$\n",
    "\n",
    "$$\n",
    "h(x) = j(x)^2 = (2|x + y|)^2 = 4(x+y)^2\n",
    "$$\n",
    "\n",
    "Simplify $( \\sqrt{|f(x)|^2} ) and ( \\sqrt{|g(x)|^2} ):$\n",
    "\n",
    "$$\n",
    "\\sqrt{|f(x)|^2} = \\sqrt{(2x+1)^2} = |2x+1|\n",
    "$$\n",
    "\n",
    "$$\n",
    "\\sqrt{|g(x)|^2} = \\sqrt{(2y-1)^2} = |2y-1|\n",
    "$$\n",
    "\n",
    "\n",
    "Rewrite the given inequality using the expressions:\n",
    "\n",
    "$$\n",
    "|2x+1| \\geq \\sqrt{4(x+y)^2} - |2y-1|\n",
    "$$\n",
    "\n",
    "$$\n",
    "|2x+1| \\geq 2|x+y| - |2y-1|\n",
    "$$\n",
    "\n",
    "Since \\( x \\) and \\( y \\) are positive integers, \\( |2x+1| \\) and \\( |2y-1| \\) are always positive, we can remove the absolute value signs:\n",
    "\n",
    "$$\n",
    "2x+1 \\geq 2|x+y| - 2y+1\n",
    "$$\n",
    "\n",
    "Solve this inequality:\n",
    "\n",
    "$$\n",
    "2x + 1 \\geq 2|x + y| - 2y + 1\n",
    "$$\n",
    "\n",
    "$$\n",
    "2x + 1 + 2y - 1 \\geq 2|x + y|\n",
    "$$\n",
    "\n",
    "$$\n",
    "2(x + y) \\geq 2|x + y|\n",
    "$$\n",
    "\n",
    "Since \\( x \\) and \\( y \\) are positive integers, \\( x + y \\) is always positive, so \\( |x + y| = x + y \\). Therefore:\n",
    "\n",
    "$$\n",
    "2(x + y) \\geq 2(x + y)\n",
    "$$\n",
    "\n",
    "Which is always true. Hence, the given inequality holds true for all positive integers \\( x \\) and \\( y \\).\n"
   ]
  },
  {
   "cell_type": "markdown",
   "metadata": {},
   "source": [
    "**2.**\n",
    "\n",
    "Given that $(u_i)$ and $(v_i)$ are square roots of even integers, we can express them as $ (u_i = \\sqrt{a_i}) $ and $ (v_i = \\sqrt{b_i}) $, where $(a_i)$ and $(b_i)$ are even integers.\n",
    "\n",
    "Expanding both sides of the inequality:\n",
    "\n",
    "Left-hand side:\n",
    "\n",
    "$$\n",
    "\\frac{\\left(\\sum_{i=1}^n u_i\\right)^2}{\\sum_{i=1}^n v_i} \\\\\n",
    "= \\frac{\\left(\\sum_{i=1}^n \\sqrt{a_i}\\right)^2}{\\sum_{i=1}^n \\sqrt{b_i}} \\\\\n",
    "= \\frac{\\left(\\sqrt{\\sum_{i=1}^n a_i}\\right)^2}{\\sqrt{\\sum_{i=1}^n b_i}} \\\\\n",
    "= \\frac{\\sum_{i=1}^n a_i}{\\sqrt{\\sum_{i=1}^n b_i}}\n",
    "$$\n",
    "\n",
    "Right-hand side:\n",
    "\n",
    "$$\n",
    "\\sum_{i=1}^n \\frac{(u_i)^2}{v_i} \\\\\n",
    "= \\sum_{i=1}^n \\frac{a_i}{\\sqrt{b_i}}\n",
    "$$\n",
    "\n",
    "Prove the inequality $(\\frac{\\sum_{i=1}^n a_i}{\\sqrt{\\sum_{i=1}^n b_i}} \\leq \\sum_{i=1}^n \\frac{a_i}{\\sqrt{b_i}})$, use the Cauchy-Schwarz Inequality.\n",
    "\n",
    "For vectors $(\\mathbf{x} = (\\sqrt{a_1}, \\sqrt{a_2}, ..., \\sqrt{a_n}))$ and $(\\mathbf{y} = (\\frac{1}{\\sqrt{b_1}}, \\frac{1}{\\sqrt{b_2}}, ..., \\frac{1}{\\sqrt{b_n}}))$, the Cauchy-Schwarz Inequality states:\n",
    "\n",
    "$$\n",
    "\\left(\\sum_{i=1}^n x_i y_i\\right)^2 \\leq \\left(\\sum_{i=1}^n x_i^2\\right) \\left(\\sum_{i=1}^n y_i^2\\right)\n",
    "$$\n",
    "\n",
    "Applying this to our case:\n",
    "\n",
    "$$\n",
    "\\left(\\sum_{i=1}^n \\sqrt{a_i} \\cdot \\frac{1}{\\sqrt{b_i}}\\right)^2 \\leq \\left(\\sum_{i=1}^n (\\sqrt{a_i})^2\\right) \\left(\\sum_{i=1}^n \\left(\\frac{1}{\\sqrt{b_i}}\\right)^2\\right) \\\\\n",
    "\\left(\\sum_{i=1}^n \\frac{a_i}{\\sqrt{b_i}}\\right)^2 \\leq \\left(\\sum_{i=1}^n a_i\\right) \\left(\\sum_{i=1}^n \\frac{1}{b_i}\\right)\n",
    "$$\n",
    "\n",
    "Now, because $(a_i)$ and $(b_i)$ are even integers, $(\\frac{1}{b_i})$ is always positive, so $(\\sum_{i=1}^n \\frac{1}{b_i})$ is also positive. Therefore:\n",
    "\n",
    "$$\n",
    "\\left(\\sum_{i=1}^n \\frac{a_i}{\\sqrt{b_i}}\\right)^2 \\leq \\left(\\sum_{i=1}^n a_i\\right) \\left(\\sum_{i=1}^n \\frac{1}{b_i}\\right) \\\\\n",
    "\\sum_{i=1}^n \\frac{a_i}{\\sqrt{b_i}} \\leq \\sqrt{\\left(\\sum_{i=1}^n a_i\\right) \\left(\\sum_{i=1}^n \\frac{1}{b_i}\\right)}\n",
    "$$\n",
    "\n",
    "This implies:\n",
    "\n",
    "$$\n",
    "\\frac{\\sum_{i=1}^n a_i}{\\sqrt{\\sum_{i=1}^n b_i}} \\leq \\sum_{i=1}^n \\frac{a_i}{\\sqrt{b_i}}\n",
    "$$\n",
    "\n",
    "Therefore, Sedrakyan's Lemma is proven.\n"
   ]
  }
 ],
 "metadata": {
  "kernelspec": {
   "display_name": "base",
   "language": "python",
   "name": "python3"
  },
  "language_info": {
   "codemirror_mode": {
    "name": "ipython",
    "version": 3
   },
   "file_extension": ".py",
   "mimetype": "text/x-python",
   "name": "python",
   "nbconvert_exporter": "python",
   "pygments_lexer": "ipython3",
   "version": "3.11.7"
  }
 },
 "nbformat": 4,
 "nbformat_minor": 2
}
